LeanYjs/Integrate/Loop.lean
@@ -1,0 +1,60 @@
+import LeanYjs.Item
+import LeanYjs.ItemOrder
+import LeanYjs.YjsArray
+import LeanYjs.Integrate
+
+variable {A : Type}
+variable [DecidableEq A]
+
+def offsetToIndex (leftIdx : ℤ) (rightIdx : ℤ) (offset : Option ℕ) (isBreak : Bool) : ℕ :=
+  let back := if isBreak then 1 else 0
+  match offset with
+  | none => rightIdx.toNat - back
+  | some o => (leftIdx + o).toNat - back
+
+def isBreak (state : ForInStep (MProd ℤ Bool)) : Bool :=
+  match state with
+  | ForInStep.done _ => true
+  | ForInStep.yield _ => false
+
+def isDone (state : ForInStep (MProd ℤ Bool)) (x : Option ℕ) : Bool :=
+  (match x with
+  | none => true
+  | some _ => false) ||
+  match state with
+  | ForInStep.done _ => true
+  | ForInStep.yield _ => false
+
+def extGetElemExcept (arr : Array (YjsItem A)) (idx : Int) : Except IntegrateError (YjsPtr A) :=
+  if idx = -1 then
+    Except.ok YjsPtr.first
+  else if idx = arr.size then
+    Except.ok YjsPtr.last
+  else
+    if idx < 0 || idx >= arr.size then
+      Except.error IntegrateError.notFound
+    else
+      match arr[idx.toNat]? with
+      | some item => return item
+      | none => Except.error IntegrateError.notFound
+
+def loopInv (arr : Array (YjsItem A)) (newItem : YjsItem A) (leftIdx : ℤ) (rightIdx : ℤ)
+    (x : Option ℕ) (state : ForInStep (MProd ℤ Bool)) :=
+  -- when x is none, we are done so current is rightIdx
+  -- when break from loop, current goes back by 1
+  let current := offsetToIndex leftIdx rightIdx x (isBreak state)
+  let ⟨ dest, scanning ⟩ := state.value
+  let done := isDone state x
+  (match x with
+    | none => True
+    | some x => 0 < x ∧ x < rightIdx - leftIdx) ∧
+  (dest ≤ current) ∧
+  (!scanning → !done -> dest = current) ∧
+  let dest := dest.toNat;
+  (∀ i : ℕ, i < dest -> (h_i_lt : i < arr.size) -> YjsLt' (A := A) arr[i] newItem) ∧
+  (∀ i, (h_dest_i : dest ≤ i) -> (h_i_c : i < current) ->
+    ∃ (i_lt_size : i < arr.size) (h_dest_lt : dest < arr.size),
+      (arr[i].origin = newItem.origin ∧ newItem.id < arr[i].id ∨
+        YjsLeq' (A := A) arr[dest] arr[i].origin)) ∧
+  (scanning -> ∃ h_dest_lt : dest < arr.size, arr[dest].origin = newItem.origin) ∧
+  (done -> ∀ item : YjsPtr A, extGetElemExcept arr current = Except.ok item -> YjsLt' (A := A) newItem item)
