LeanYjs/YjsArray/ArrSet.lean
@@ -1,0 +1,140 @@
+import Mathlib.Tactic.ApplyAt
+
+import LeanYjs.Item
+import LeanYjs.ItemSet
+
+variable {A : Type}
+
+def ArrSet (arr : List (YjsItem A)) : YjsPtr A -> Prop :=
+  fun a => match a with
+  | YjsPtr.itemPtr item => item ∈ arr
+  | YjsPtr.first => True
+  | YjsPtr.last => True
+
+def ArrSetClosed (arr : List (YjsItem A)) : Prop :=
+  IsClosedItemSet (ArrSet arr)
+
+theorem subset_ArrSet {arr1 arr2 : Array (YjsItem A)} {a : YjsPtr A}:
+  (∀ a, a ∈ arr1 -> a ∈ arr2)
+  -> ArrSet arr1.toList a
+  -> ArrSet arr2.toList a := by
+  intros h_subset h_arr1
+  simp [ArrSet] at *
+  cases a with
+  | first => simp
+  | last => simp
+  | itemPtr a =>
+    simp at *
+    apply h_subset a h_arr1
+
+theorem arr_set_closed_push (arr : List (YjsItem A)) (item : YjsItem A) :
+  ArrSetClosed arr ->
+  ArrSet arr item.origin ->
+  ArrSet arr item.rightOrigin ->
+  ArrSetClosed (item :: arr) := by
+  intros hclosed horigin hright
+  constructor <;> try simp [ArrSet]
+  . intros o r id c hor
+    cases o with
+    | itemPtr item' =>
+      simp
+      cases hor with
+      | inr hitem =>
+        right
+        apply hclosed.closedLeft at hitem
+        assumption
+      | inl heq =>
+        subst heq
+        right
+        assumption
+    | first =>
+      simp
+    | last =>
+      simp
+  . intros o r id c hor
+    cases r with
+    | itemPtr item' =>
+      simp
+      cases hor with
+      | inr hitem =>
+        right
+        apply hclosed.closedRight at hitem
+        assumption
+      | inl heq =>
+        subst heq
+        right
+        assumption
+    | first =>
+      simp
+    | last =>
+      simp
+
+theorem arr_set_item_exists_index (arr arr' : List (YjsItem A)) (item : YjsItem A) :
+  ArrSetClosed arr' ->
+  ArrSet arr item ->
+  (∃ l, l ++ arr = arr') ->
+  ∃ i : Fin arr.length, arr[i] = item := by
+  intros hclosed hitem hsublist
+  induction arr with
+  | nil =>
+    simp [ArrSet] at hitem
+  | cons head arr ih =>
+    simp [ArrSet] at hitem
+    cases hitem with
+    | inl heq =>
+      subst heq
+      have zero_lt_len : 0 < (item :: arr).length := by simp
+      exists Fin.mk 0 zero_lt_len
+    | inr hin =>
+      have hsublist' : ∃ l', l' ++ arr = arr' := by
+        obtain ⟨ l, heq ⟩ := hsublist
+        exists (l ++ [head])
+        rw [List.append_assoc]
+        simp; assumption
+      obtain ⟨ i, hi ⟩ := ih hin hsublist'
+      let i' : Fin ((head :: arr).length) := by
+        simp
+        apply Fin.addNat i 1
+      exists i'
+
+theorem arr_set_closed_exists_index_for_origin :
+  ∀ (arr : List (YjsItem A)) (item : YjsItem A),
+  ArrSetClosed arr ->
+  ArrSet arr item ->
+  item.origin = YjsPtr.first ∨ item.origin = YjsPtr.last ∨ ∃ i : Fin arr.length, arr[i] = item.origin := by
+  intros arr item hclosed hitem
+  obtain ⟨ o, r, id, c ⟩ := item
+  apply hclosed.closedLeft at hitem
+  simp [YjsItem.origin]
+  cases o with
+  | first =>
+    left; simp
+  | last =>
+    right; left; simp
+  | itemPtr o =>
+    right; right
+    obtain ⟨ i, h ⟩ := arr_set_item_exists_index arr arr o hclosed hitem (by exists [])
+    exists i
+    simp
+    assumption
+
+theorem arr_set_closed_exists_index_for_right_origin :
+  ∀ (arr : List (YjsItem A)) (item : YjsItem A),
+  ArrSetClosed arr ->
+  ArrSet arr item ->
+  item.rightOrigin = YjsPtr.first ∨ item.rightOrigin = YjsPtr.last ∨ ∃ i : Fin arr.length, arr[i] = item.rightOrigin := by
+  intros arr item hclosed hitem
+  obtain ⟨ o, r, id, c ⟩ := item
+  apply hclosed.closedRight at hitem
+  simp [YjsItem.rightOrigin]
+  cases r with
+  | first =>
+    left; simp
+  | last =>
+    right; left; simp
+  | itemPtr o =>
+    right; right
+    obtain ⟨ i, h ⟩ := arr_set_item_exists_index arr arr o hclosed hitem (by exists [])
+    exists i
+    simp
+    assumption
