LeanYjs/YjsArray/Invariant.lean
@@ -1,0 +1,366 @@
+import LeanYjs.ListLemmas
+import LeanYjs.Item
+import LeanYjs.ItemSet
+import LeanYjs.ClientId
+import LeanYjs.ItemOrder
+import LeanYjs.ItemSetInvariant
+import LeanYjs.Totality
+import LeanYjs.Transitivity
+import LeanYjs.Asymmetry
+import LeanYjs.Integrate
+import LeanYjs.YjsArray.ArrSet
+
+structure YjsArrInvariant (arr : List (YjsItem A)) : Prop where
+  closed : IsClosedItemSet (ArrSet arr)
+  item_set_inv : ItemSetInvariant (ArrSet arr)
+  sorted : List.Pairwise (fun (x y : YjsItem A) => YjsLt' (A := A) x y) arr
+  unique : List.Pairwise (fun x y => x ≠ y) arr
+
+section YjsArrInvariant
+
+variable [DecidableEq A]
+
+theorem same_yjs_set_unique_aux (xs_all ys_all xs ys : List (YjsItem A)) :
+  YjsArrInvariant xs_all ->
+  YjsArrInvariant ys_all ->
+  (∀ a, ArrSet xs_all a ↔ ArrSet ys_all a) ->
+  (∃ t, t ++ xs = xs_all) ->
+  (∃ t, t ++ ys = ys_all) ->
+  (∀ x, ArrSet xs x ↔ ArrSet ys x) ->
+  xs = ys := by
+  intros hinv1 hinv2 hseteq_all hsubset1 hsubset2 hseteq
+  obtain ⟨ hclosed1, hinv1, hsort1, huniq1 ⟩ := hinv1
+  obtain ⟨ hclosed2, hinv2, hsort2, huniq2 ⟩ := hinv2
+
+  revert ys
+
+  induction xs with
+  | nil =>
+    intros ys hsubset2 hseteq
+    cases ys with
+    | nil => eq_refl
+    | cons y ys =>
+      obtain hitem := hseteq y
+      simp [ArrSet] at hitem
+  | cons x xs ih =>
+    intros ys hsubset2 hseteq
+    cases ys with
+    | nil =>
+      obtain hitem := hseteq x
+      simp [ArrSet] at hitem
+    | cons y ys =>
+      have hmin1 : ∀ a ∈ xs, YjsLt' (A := A) x a := by
+        obtain ⟨ t, heq ⟩ := hsubset1
+        subst heq
+        rw [List.pairwise_append] at hsort1
+        obtain ⟨ _, hsort1, _ ⟩ := hsort1
+        simp at hsort1
+        obtain ⟨ hsort1, _ ⟩ := hsort1
+        assumption
+      have hmin2 : ∀ a ∈ ys, YjsLt' (A := A) y a := by
+        obtain ⟨ t, heq ⟩ := hsubset2
+        subst heq
+        rw [List.pairwise_append] at hsort2
+        obtain ⟨ _, hsort2, _ ⟩ := hsort2
+        simp at hsort2
+        obtain ⟨ hsort2, _ ⟩ := hsort2
+        assumption
+
+      have heq : x = y := by
+        have hlt1 : x = y ∨ YjsLt' (A := A) y x := by
+          by_cases heq : x = y
+          . left; assumption
+          . obtain ⟨ hinx, _ ⟩ := hseteq x
+            have hinx : x = y ∨ x ∈ ys := by
+              simp [ArrSet] at hinx
+              assumption
+            cases hinx with
+            | inl heq =>
+              left; assumption
+            | inr hinx =>
+              apply hmin2 at hinx
+              obtain ⟨ _, hinx ⟩ := hinx
+              right
+              constructor
+              assumption
+
+        have hlt2 : x = y ∨ YjsLt' (A := A) x y := by
+          by_cases heq : x = y
+          . subst heq; left; eq_refl
+          . obtain ⟨ _, hinx ⟩ := hseteq y
+            have hiny : y = x ∨ y ∈ xs := by
+              simp [ArrSet] at hinx
+              assumption
+            cases hiny with
+            | inl heq =>
+              subst heq; left; eq_refl
+            | inr hiny =>
+              apply hmin1 at hiny
+              obtain ⟨ _, hiny ⟩ := hiny
+              right
+              constructor
+              assumption
+
+        cases hlt1 with
+        | inl heq =>
+          assumption
+        | inr hlt1 =>
+          cases hlt2 with
+          | inl heq =>
+            assumption
+          | inr hlt2 =>
+            obtain ⟨ tx, heq1 ⟩ := hsubset1
+            obtain ⟨ ty, heq2 ⟩ := hsubset2
+            subst heq1 heq2
+            cases yjs_lt_asymm hclosed2 hinv2 x y (by rw [<-hseteq_all]; simp [ArrSet]) (by simp [ArrSet]) hlt2 hlt1
+
+      subst heq
+      congr
+
+      apply ih
+      . obtain ⟨ t, heq ⟩ := hsubset1
+        subst heq
+        exists (t ++ [x])
+        simp
+      . obtain ⟨ t, heq ⟩ := hsubset2
+        subst heq
+        exists (t ++ [x])
+        simp
+      . intros a
+        simp [ArrSet] at *
+        cases a with
+        | first =>
+          simp
+        | last =>
+          simp
+        | itemPtr a =>
+          specialize hseteq a
+          simp at *
+          obtain ⟨ t, heq ⟩ := hsubset1
+          subst heq
+          obtain ⟨ t', heq ⟩ := hsubset2
+          subst heq
+          rw [List.pairwise_append] at huniq1
+          rw [List.pairwise_append] at huniq2
+          simp at *
+          obtain ⟨ _, ⟨ huniq1, _ ⟩, _ ⟩ := huniq1
+          obtain ⟨ _, ⟨ huniq2, _ ⟩ , _ ⟩ := huniq2
+          constructor
+          . intros hin
+            obtain hneq := huniq1 _ hin
+            have h : a = x ∨ a ∈ ys := by
+              rw [<-hseteq]
+              right; assumption
+            cases h with
+            | inl heq =>
+              subst heq
+              cases hneq (refl _)
+            | inr hin =>
+              assumption
+          . intros hin
+            obtain hneq := huniq2 _ hin
+            have h : a = x ∨ a ∈ xs := by
+              rw [hseteq]
+              right; assumption
+            cases h with
+            | inl heq =>
+              subst heq
+              cases hneq (refl _)
+            | inr hin =>
+              assumption
+
+theorem same_yjs_set_unique (xs ys : List (YjsItem A)) :
+  YjsArrInvariant xs ->
+  YjsArrInvariant ys ->
+  (∀ a, ArrSet xs a ↔ ArrSet ys a) ->
+  xs = ys := by
+  intros hinv1 hinv2 hseteq
+  apply same_yjs_set_unique_aux xs ys xs ys hinv1 hinv2 hseteq
+  . exists []
+  . exists []
+  . apply hseteq
+
+end YjsArrInvariant
+
+theorem insertIdxIfInBounds_mem {arr : Array (YjsItem A)} :
+  i ≤ arr.size →
+  (ArrSet (newItem :: arr.toList) x ↔ ArrSet (arr.insertIdxIfInBounds i newItem).toList x) := by
+  intros hlt
+  simp [ArrSet]
+  cases x <;> try simp
+  rw [List.insertIdxIfInBounds_toArray]
+  simp
+  rw [List.mem_insertIdx]
+  simp
+  assumption
+
+theorem YjsArrInvariant_insertIdxIfInBounds [DecidableEq A] (arr : Array (YjsItem A)) (newItem : YjsItem A) (i : ℕ) :
+  IsClosedItemSet (ArrSet $ newItem :: arr.toList)
+  -> ItemSetInvariant (ArrSet $ newItem :: arr.toList)
+  -> YjsArrInvariant arr.toList
+  -> (hisize : i ≤ arr.size)
+  -> ((hizero : 0 < i) -> YjsLt' (A := A) arr[i - 1] newItem)
+  -> ((hisize : i < arr.size) -> YjsLt' (A := A) newItem arr[i])
+  -> (∀ a, a ∈ arr -> a ≠ newItem)
+  -> YjsArrInvariant (arr.insertIdxIfInBounds i newItem).toList := by
+  intros hclosed hinv harrinv hisize hlt1 hlt2 hneq
+  obtain ⟨ _, _, hsorted, hunique ⟩ := harrinv
+  have heqset : ∀ x, ArrSet (newItem :: arr.toList) x ↔ ArrSet (List.insertIdx arr.toList i newItem) x := by
+    intros x
+    simp only [ArrSet]
+    cases x with
+    | first => simp
+    | last => simp
+    | itemPtr x =>
+      simp
+      rw [List.mem_insertIdx hisize]
+      simp
+
+  have heqset' : ∀ x, ArrSet (newItem :: arr.toList) x ↔ ArrSet (arr.insertIdxIfInBounds i newItem).toList x := by
+    intros
+    rw [List.insertIdxIfInBounds_toArray]
+    simp
+    rw [heqset]
+
+  have hsubset a : (ArrSet arr.toList) a -> (ArrSet (List.insertIdx arr.toList i newItem)) a := by
+    intros hmem
+    cases a with
+    | first => simp [ArrSet]
+    | last => simp [ArrSet]
+    | itemPtr a =>
+      simp [ArrSet]
+      rw [List.mem_insertIdx hisize]
+      right
+      assumption
+
+  have hsubset' : ∀ x, ArrSet arr.toList x -> ArrSet (newItem :: arr.toList) x := by
+    intros a hmem
+    simp [ArrSet] at *
+    cases a <;> simp
+    right
+    assumption
+
+  apply YjsArrInvariant.mk
+  . apply IsClosedItemSet.eq_set (P := ArrSet $ newItem :: arr.toList) _ hclosed heqset'
+  . apply ItemSetInvariant.eq_set (P := ArrSet $ newItem :: arr.toList) _ hclosed hinv heqset'
+  . rw [List.insertIdxIfInBounds_toArray]
+    simp
+    apply List.Pairwise_insertIdx
+    . apply List.Pairwise_weaken (R := fun (a b : YjsItem A) => YjsLt' (A := A) a b) <;> try assumption
+      intros
+      assumption
+    . intros j hji
+      apply yjs_leq'_p_trans1 (inv := hinv) (y := arr[i - 1]) <;> try assumption
+      . simp [ArrSet]
+      . simp [ArrSet]
+      . simp [ArrSet]
+      . rw [List.pairwise_iff_getElem] at hsorted
+        cases Nat.lt_or_ge j (i - 1) with
+        | inl hj_lt =>
+          have hlt : YjsLt' (A := A) (YjsPtr.itemPtr arr[j]) (YjsPtr.itemPtr arr[i - 1]) := by
+            apply hsorted; assumption
+          obtain ⟨ k, hlt ⟩ := hlt
+          simp at *
+          -- We can't use `exists k + 1` because it causes error in Lean4.18-rc1.
+          -- This `apply` generates a seemingly unnecesarry goal here.
+          apply Exists.intro (k + 1)
+          apply YjsLeq.leqLt
+          assumption
+          -- Here, we need to prove the following:
+          --- List.Pairwise (fun x y => x ≠ y) arr.toList →
+          -- (∀ (x : YjsPtr A), ArrSet (newItem :: arr.toList) x ↔ ArrSet (List.insertIdx i newItem arr.toList) x) →
+          --   (∀ (x : YjsPtr A), ArrSet (newItem :: arr.toList) x ↔ ArrSet (arr.insertIdxIfInBounds i newItem).toList x) →
+          --     (∀ (a : YjsPtr A), ArrSet arr.toList a → ArrSet (List.insertIdx i newItem arr.toList) a) →
+          --       (∀ (x : YjsPtr A), ArrSet arr.toList x → ArrSet (newItem :: arr.toList) x) → i ≤ arr.toList.length
+          intros
+          simp; omega
+        | inr hj_ge =>
+          have heq : j = i - 1 := by omega
+          subst heq
+          simp
+          exists 0
+          apply YjsLeq.leqSame
+      . apply hlt1; omega
+    . intros j hij hjlen
+      simp at hjlen
+      apply yjs_leq'_p_trans2 (inv := hinv) (y := YjsPtr.itemPtr arr[i]) <;> try assumption
+      . simp [ArrSet]
+      . simp [ArrSet]
+      . simp [ArrSet]
+      . apply hlt2
+      . rw [List.pairwise_iff_getElem] at hsorted
+        cases Nat.lt_or_ge i j with
+        | inl hj_lt =>
+          have hlt : YjsLt' (A := A) (YjsPtr.itemPtr arr[i]) (YjsPtr.itemPtr arr[j]) := by
+            apply hsorted; try assumption
+          obtain ⟨ h, hlt' ⟩ := hlt
+          exists h + 1; right; assumption
+        | inr hj_ge =>
+          have heq : j = i := by omega
+          subst heq
+          simp
+          exists 0; apply YjsLeq.leqSame
+  . rw [List.insertIdxIfInBounds_toArray]
+    apply List.Pairwise_insertIdx <;> try assumption
+    . intros
+      apply hneq
+      simp
+    . intros j hij hlt heq
+      apply hneq arr[j]
+      simp
+      subst heq
+      simp
+
+theorem item_set_invariant_push (item : YjsItem A) :
+  ItemSetInvariant (ArrSet arr) →
+  ArrSetClosed arr →
+  YjsLt' item.origin item.rightOrigin →
+  (∀ x, OriginReachable item x → YjsLeq' x item.origin ∨ YjsLeq' item.rightOrigin x) →
+  (∀ x : YjsItem A, ArrSet arr x → x.id = item.id → YjsLeq' x item.origin ∨ YjsLeq' item.rightOrigin x) →
+  ItemSetInvariant (ArrSet (item :: arr)) := by
+  intros hinv hclosed horigin hreach hsameid
+  constructor
+  · intros o r c id hitem
+    simp [ArrSet] at hitem
+    cases hitem with
+    | inr hin =>
+      apply hinv.origin_not_leq at hin
+      assumption
+    | inl heq =>
+      subst heq
+      assumption
+  · intros o r c id x hin hreachable
+    simp [ArrSet] at hin
+    cases hin with
+    | inr hin =>
+      apply hinv.origin_nearest_reachable _ _ _ _ _ hin hreachable
+    | inl heq =>
+      subst heq
+      simp [YjsItem.origin, YjsItem.rightOrigin] at *
+      apply hreach _ hreachable
+  · intros x y hinx hiny hineq hid
+    simp [ArrSet] at *
+    cases hinx with
+    | inr hinx =>
+      cases hiny with
+      | inr hiny =>
+        apply hinv.same_id_ordered _ _ hinx hiny hineq hid
+      | inl hleq =>
+        subst hleq
+        cases hsameid _ hinx hid with
+        | inl hleq =>
+          left; assumption
+        | inr hleq =>
+          right; right; right; assumption
+    | inl hinx =>
+      subst hinx
+      cases hiny with
+      | inr hiny =>
+        cases hsameid _ hiny (by rw [hid]) with
+        | inl hleq =>
+          right; left; assumption
+        | inr hleq =>
+          right; right; left; assumption
+      | inl heqy =>
+        subst heqy
+        cases hineq (rfl)
